libcrux-ml-kem/proofs/fstar/spec/Spec.MLKEM.fst
@@ -295,7 +295,7 @@ val ind_cpa_generate_keypair (r:rank) (randomness:t_Array u8 v_CPA_KEY_GENERATIO
                              t_MLKEMCPAKeyPair r
 let ind_cpa_generate_keypair r randomness =
     let hashed = v_G randomness in
-    let (seed_for_A, seed_for_secret_and_error) = split hashed (sz 32) in
+      let (seed_for_A, seed_for_secret_and_error) = split hashed (sz 32) in
     let matrix_A_as_ntt = sample_matrix_A_ntt #r seed_for_A in
     let secret_as_ntt = sample_vector_cbd_then_ntt #r seed_for_secret_and_error (sz 0) in
     let error_as_ntt = sample_vector_cbd_then_ntt #r seed_for_secret_and_error r in
